ok

SStructTT/SStruct/Erasure/Substitution.lean
@@ -1,51 +1,56 @@
-import SStructTT.SStruct.Static.Substitution
-import SStructTT.SStruct.Dynamic.Renaming
-open SStruct.Static
+import SStructTT.SStruct.Dynamic.Substitution
+import SStructTT.SStruct.Erasure.Renaming
+open SStruct.Dynamic
 
-namespace SStruct.Dynamic
+namespace SStruct.Erasure
 variable {Srt : Type} [ord : SrtOrder Srt]
 
 @[aesop safe (rule_sets := [subst]) [constructors]]
-inductive AgreeSubst : (Var -> Tm Srt) ->
+inductive AgreeSubst :
+  (Var -> SStruct.Tm Srt) ->
+  (Var -> Erasure.Tm Srt) ->
   Static.Ctx Srt -> Dynamic.Ctx Srt ->
   Static.Ctx Srt -> Dynamic.Ctx Srt -> Prop
 where
-  | nil {σ} :
-    AgreeSubst σ [] [] [] []
-  | cons {Γ Γ' Δ Δ' A} r {s i σ} :
+  | nil {σ σ'} :
+    AgreeSubst σ σ' [] [] [] []
+  | cons {Γ Γ' Δ Δ' A} r {s i σ σ'} :
     Γ ⊢ A : .srt s i ->
-    AgreeSubst σ Γ Δ Γ' Δ' ->
-    AgreeSubst (up σ) (A :: Γ) (A :⟨r, s⟩ Δ) (A.[σ] :: Γ') (A.[σ] :⟨r, s⟩ Δ')
-  | wk_im {Γ Γ' Δ Δ' A m s σ} :
+    AgreeSubst σ σ' Γ Δ Γ' Δ' ->
+    AgreeSubst (up σ) (up σ') (A :: Γ) (A :⟨r, s⟩ Δ) (A.[σ] :: Γ') (A.[σ] :⟨r, s⟩ Δ')
+  | wk_im {Γ Γ' Δ Δ' A m m' s σ σ'} :
     Γ' ⊢ m : A.[σ] ->
-    AgreeSubst σ Γ Δ Γ' Δ' ->
-    AgreeSubst (m .: σ) (A :: Γ) (A :⟨.im, s⟩ Δ) Γ' Δ'
-  | wk_ex {Γ Γ' Δ Δ' Δa Δb A m s σ} :
+    AgreeSubst σ σ' Γ Δ Γ' Δ' ->
+    AgreeSubst (m .: σ) (m' .: σ') (A :: Γ) (A :⟨.im, s⟩ Δ) Γ' Δ'
+  | wk_ex {Γ Γ' Δ Δ' Δa Δb A m m' s σ σ'} :
     Merge Δa Δb Δ' ->
     Δa ≤* s ->
-    Γ' ;; Δa ⊢ m : A.[σ] ->
-    AgreeSubst σ Γ Δ Γ' Δb ->
-    AgreeSubst (m .: σ) (A :: Γ) (A :⟨.ex, s⟩ Δ) Γ' Δ'
-  | conv {Γ Γ' Δ Δ' A B r s i σ} :
+    Γ' ;; Δa ⊢ m ▷ m' : A.[σ] ->
+    AgreeSubst σ σ' Γ Δ Γ' Δb ->
+    AgreeSubst (m .: σ) (m' .: σ') (A :: Γ) (A :⟨.ex, s⟩ Δ) Γ' Δ'
+  | conv {Γ Γ' Δ Δ' A B r s i σ σ'} :
     A === B ->
     Γ ⊢ B : .srt s i ->
     Γ' ⊢ B.[shift 1].[σ] : .srt s i ->
-    AgreeSubst σ (A :: Γ) (A :⟨r, s⟩ Δ) Γ' Δ' ->
-    AgreeSubst σ (B :: Γ) (B :⟨r, s⟩ Δ) Γ' Δ'
+    AgreeSubst σ σ' (A :: Γ) (A :⟨r, s⟩ Δ) Γ' Δ' ->
+    AgreeSubst σ σ' (B :: Γ) (B :⟨r, s⟩ Δ) Γ' Δ'
 
-lemma AgreeSubst.toStatic {Γ Γ'} {Δ Δ' : Ctx Srt} {σ} :
-    Dynamic.AgreeSubst σ Γ Δ Γ' Δ' -> Static.AgreeSubst σ Γ Γ' := by
+lemma AgreeSubst.toDynamic {Γ Γ'} {Δ Δ' : Ctx Srt} {σ σ'} :
+    Erasure.AgreeSubst σ σ' Γ Δ Γ' Δ' -> Dynamic.AgreeSubst σ Γ Δ Γ' Δ' := by
   intro agr
   induction agr <;> try aesop (rule_sets := [subst])
   case cons => constructor <;> assumption
   case wk_im => constructor <;> assumption
   case wk_ex tym agr ih =>
-    constructor
-    . apply tym.toStatic
-    . assumption
+    constructor <;> try assumption
+    apply tym.toDynamic
+
+lemma AgreeSubst.toStatic {Γ Γ'} {Δ Δ' : Ctx Srt} {σ σ'} :
+    Erasure.AgreeSubst σ σ' Γ Δ Γ' Δ' -> Static.AgreeSubst σ Γ Γ' := by
+  intro agr; apply agr.toDynamic.toStatic
 
 @[aesop safe (rule_sets := [subst])]
-lemma AgreeSubst.refl {Γ} {Δ : Ctx Srt} : Γ ;; Δ ⊢ -> AgreeSubst ids Γ Δ Γ Δ := by
+lemma AgreeSubst.refl {Γ} {Δ : Ctx Srt} : Γ ;; Δ ⊢ -> AgreeSubst ids ids Γ Δ Γ Δ := by
   intro wf; induction wf
   all_goals try trivial
   case nil => constructor
@@ -54,36 +59,22 @@ lemma AgreeSubst.refl {Γ} {Δ : Ctx Srt} : Γ ;; Δ ⊢ -> AgreeSubst ids Γ Δ
     asimp at agr; assumption
 
 @[aesop safe (rule_sets := [subst])]
-lemma AgreeSubst.implicit {Γ Γ'} {Δ Δ' : Ctx Srt} {σ} :
-    AgreeSubst σ Γ Δ Γ' Δ' ->
+lemma AgreeSubst.implicit {Γ Γ'} {Δ Δ' : Ctx Srt} {σ σ'} :
+    AgreeSubst σ σ' Γ Δ Γ' Δ' ->
     Δ.Forall (∃ A s, . = (A, .im, s)) ->
     Δ'.Forall (∃ A s, . = (A, .im, s)) := by
-  intro agr h; induction agr
-  case nil => simp
-  case cons ih => simp at h; aesop
-  case wk_im ih => simp at h; aesop
-  case wk_ex => simp at h
-  case conv => simp at h; aesop
+  intro agr; apply agr.toDynamic.implicit
 
-lemma AgreeSubst.lower {Γ Γ'} {Δ Δ' : Ctx Srt} {s σ} :
-    AgreeSubst σ Γ Δ Γ' Δ' -> Δ ≤* s -> Δ' ≤* s := by
-  intro agr lw; induction agr generalizing s
-  case nil => assumption
-  case cons =>
-    cases lw <;> constructor <;> aesop
-  case wk_im => cases lw; aesop
-  case wk_ex mrg _ _ _ _ =>
-    cases lw
-    apply mrg.lower
-    . apply Lower.trans <;> assumption
-    . aesop
-  case conv ih => cases lw <;> aesop
+lemma AgreeSubst.lower {Γ Γ'} {Δ Δ' : Ctx Srt} {s σ σ'} :
+    AgreeSubst σ σ' Γ Δ Γ' Δ' -> Δ ≤* s -> Δ' ≤* s := by
+  intro agr; apply agr.toDynamic.lower
 
-lemma AgreeSubst.has {Γ Γ'} {Δ Δ' : Ctx Srt} {A x s σ} :
-    AgreeSubst σ Γ Δ Γ' Δ' -> Γ' ;; Δ' ⊢ -> Has Δ x s A -> Γ' ;; Δ' ⊢ (σ x) : A.[σ] := by
+lemma AgreeSubst.has {Γ Γ'} {Δ Δ' : Ctx Srt} {A x s σ σ'} :
+    AgreeSubst σ σ' Γ Δ Γ' Δ' -> Γ' ;; Δ' ⊢ ->
+    Has Δ x s A -> Γ' ;; Δ' ⊢ (σ x) ▷ (σ' x) : A.[σ] := by
   intro agr wf hs; induction agr generalizing x A
   case nil => cases hs
-  case cons A r s i σ tyA agr ih =>
+  case cons A r s i σ σ' tyA agr ih =>
     cases r with
     | ex =>
       rcases hs with ⟨h⟩; asimp
@@ -95,7 +86,7 @@ lemma AgreeSubst.has {Γ Γ'} {Δ Δ' : Ctx Srt} {A x s σ} :
       rcases wf with _ | ⟨_, wf⟩
       rcases hs with _ | @⟨_, A, x, s, hs⟩; asimp
       rw[show A.[σ !> shift 1] = A.[σ].[shift 1] by asimp]
-      apply Typed.eweaken <;> try first | rfl | assumption
+      apply Erased.eweaken <;> try first | rfl | assumption
       apply ih <;> assumption
   case wk_im ih =>
     rcases hs with _ | @⟨_, A, x, s, hs⟩; asimp
@@ -104,7 +95,7 @@ lemma AgreeSubst.has {Γ Γ'} {Δ Δ' : Ctx Srt} {A x s σ} :
     rcases hs with ⟨h⟩; asimp
     rw[<-mrg.sym.implicit (agr.implicit h)]
     assumption
-  case conv r _ _  σ eq tyB tyB' agr ih =>
+  case conv r _ _  σ σ' eq tyB tyB' agr ih =>
     cases r with
     | im =>
       rcases hs with _ | @⟨_, A, x, s, hs⟩
@@ -113,22 +104,22 @@ lemma AgreeSubst.has {Γ Γ'} {Δ Δ' : Ctx Srt} {A x s σ} :
       . constructor; assumption
     | ex =>
       rcases hs with ⟨h⟩
-      apply Typed.conv
-      . apply Conv.subst _ (Conv.subst _ eq)
+      apply Erased.conv
+      . apply Static.Conv.subst _ (Static.Conv.subst _ eq)
       . apply ih wf; constructor; assumption
       . assumption
 
-lemma AgreeSubst.split {Γ Γ'} {Δ Δ' Δa Δb : Ctx Srt} {σ} :
-    AgreeSubst σ Γ Δ Γ' Δ' -> Merge Δa Δb Δ ->
+lemma AgreeSubst.split {Γ Γ'} {Δ Δ' Δa Δb : Ctx Srt} {σ σ'} :
+    AgreeSubst σ σ' Γ Δ Γ' Δ' -> Merge Δa Δb Δ ->
     ∃ Δa' Δb',
       Merge Δa' Δb' Δ' ∧
-      AgreeSubst σ Γ Δa Γ' Δa' ∧
-      AgreeSubst σ Γ Δb Γ' Δb' := by
+      AgreeSubst σ σ' Γ Δa Γ' Δa' ∧
+      AgreeSubst σ σ' Γ Δb Γ' Δb' := by
   intro agr mrg; induction agr generalizing Δa Δb
   case nil =>
     cases mrg; exists [], []
     aesop (rule_sets := [subst])
-  case cons A r s i σ tyA agr ih =>
+  case cons A r s i σ σ' tyA agr ih =>
     cases mrg with
     | contra _ _ h mrg =>
       have ⟨Δa', Δb', mrg, agr1, agr2⟩ := ih mrg
@@ -198,7 +189,7 @@ lemma AgreeSubst.split {Γ Γ'} {Δ Δ' Δa Δb : Ctx Srt} {σ} :
         . exact lw
         . exact tym
         . exact agr2
-  case conv A B r s i σ eq tyB tyB' agr ih =>
+  case conv A B r s i σ σ' eq tyB tyB' agr ih =>
     cases mrg with
     | contra _ _ h mrg =>
       have ⟨Δa', Δb', mrg', agr1, agr2⟩ := ih (Merge.contra A s h mrg)
@@ -213,113 +204,80 @@ lemma AgreeSubst.split {Γ Γ'} {Δ Δ' Δa Δb : Ctx Srt} {σ} :
       have ⟨Δa', Δb', mrg', agr1, agr2⟩ := ih (Merge.im _ _ mrg)
       exists Δa', Δb'; aesop (rule_sets := [subst])
 
-lemma AgreeSubst.wf_nil {Γ'} {Δ' : Ctx Srt} {σ} :
-    AgreeSubst σ [] [] Γ' Δ' -> Γ' ;; Δ' ⊢ := by
-  generalize e1: [] = Γ
-  generalize e2: [] = Δ
-  intro agr; induction agr <;> try trivial
-  constructor
-
-lemma AgreeSubst.wf_cons {Γ Γ'} {Δ Δ' : Ctx Srt} {A r s σ} :
-    AgreeSubst σ (A :: Γ) (A :⟨r, s⟩ Δ) Γ' Δ' -> Γ ;; Δ ⊢ ->
-    (∀ {Γ' Δ' σ}, AgreeSubst σ Γ Δ Γ' Δ' → Γ' ;; Δ' ⊢) ->
-    Γ' ;; Δ' ⊢ := by
-  generalize e1: A :: Γ = Γ0
-  generalize e2: A :⟨r, s⟩ Δ = Δ0
-  intro agr wf h; induction agr generalizing Γ Δ A r s <;> try trivial
-  case cons tyA agr ih =>
-    cases e1; cases e2
-    constructor
-    . apply tyA.substitution agr.toStatic
-    . apply h agr
-  case wk_im agr _ =>
-    cases e1; cases e2
-    apply h agr
-  case wk_ex mrg lw tym agr ih =>
-    cases e1; cases e2
-    apply Wf.merge mrg tym.toWf (h agr)
-  case conv ih =>
-    cases e1; cases e2
-    apply ih rfl rfl wf h
-
 @[aesop safe (rule_sets := [subst])]
-lemma AgreeSubst.wf {Γ Γ'} {Δ Δ' : Ctx Srt} {σ} :
-    AgreeSubst σ Γ Δ Γ' Δ' ->
+lemma AgreeSubst.wf {Γ Γ'} {Δ Δ' : Ctx Srt} {σ σ'} :
+    AgreeSubst σ σ' Γ Δ Γ' Δ' ->
     Γ ;; Δ ⊢ -> Γ' ;; Δ' ⊢ := by
-  intro agr wf; induction wf generalizing Γ' Δ' σ
-  all_goals try aesop
-  case nil => apply agr.wf_nil
-  case cons => apply agr.wf_cons <;> aesop
+  intro agr; apply agr.toDynamic.wf
 
-lemma Typed.substitution {Γ Γ'} {Δ Δ' : Ctx Srt} {A m σ} :
-    Γ ;; Δ ⊢ m : A -> AgreeSubst σ Γ Δ Γ' Δ' -> Γ' ;; Δ' ⊢ m.[σ] : A.[σ] := by
-  intro ty agr; induction ty using
-    @Typed.rec _ ord
-      (motive_2 := fun Γ Δ _ => ∀ {Γ' Δ' σ}, AgreeSubst σ Γ Δ Γ' Δ' -> Γ' ;; Δ' ⊢)
-  generalizing Γ' Δ' σ <;> asimp
-  case var wf hs ih => apply agr.has (ih agr) hs
-  case lam_im lw tyA tym ih =>
-    apply Typed.lam_im
+lemma Erased.substitution {Γ Γ'} {Δ Δ' : Ctx Srt} {A m m' σ σ'} :
+    Γ ;; Δ ⊢ m ▷ m' : A -> AgreeSubst σ σ' Γ Δ Γ' Δ' ->
+    Γ' ;; Δ' ⊢ m.[σ] ▷ m'.[σ'] : A.[σ] := by
+  intro ty agr; induction ty generalizing Γ' Δ' σ σ' <;> asimp
+  case var wf hs =>
+    apply agr.has (agr.wf wf) hs
+  case lam_im lw tyA erm ihm =>
+    apply Erased.lam_im
     . apply agr.lower lw
     . apply tyA.substitution agr.toStatic
-    . apply ih; constructor <;> assumption
-  case lam_ex A B m rA s sA i rs lw tyA tym ih =>
-    apply Typed.lam_ex
+    . apply ihm; constructor <;> assumption
+  case lam_ex A B m rA s sA i rs lw tyA erm ih =>
+    apply Erased.lam_ex
     . assumption
     . apply agr.lower lw
     . apply tyA.substitution agr.toStatic
     . apply ih; constructor <;> assumption
-  case app_im tym tyn ih =>
-    replace tym := ih agr; asimp at tym
+  case app_im erm tyn ih =>
+    replace erm := ih agr; asimp at erm
     replace tyn := tyn.substitution agr.toStatic
-    have ty := Typed.app_im tym tyn
-    asimp at ty; assumption
-  case app_ex mrg tym tyn ihm ihn =>
+    have er := Erased.app_im erm tyn
+    asimp at er; assumption
+  case app_ex mrg erm ern ihm ihn =>
     have ⟨Δa, Δb, mrg, agr1, agr2⟩ := agr.split mrg
     specialize ihm agr1; asimp at ihm
     specialize ihn agr2
-    have ty := Typed.app_ex mrg ihm ihn
-    asimp at ty; assumption
-  case tup_im B m n s i tyS tym tyn ihm =>
+    have er := Erased.app_ex mrg ihm ihn
+    asimp at er; assumption
+  case tup_im B m m' n s i tyS erm tyn ihm =>
     replace tyS := tyS.substitution agr.toStatic; asimp at tyS
-    replace tym := ihm agr; asimp at tym
+    replace erm := ihm agr; asimp at erm
     replace tyn := tyn.substitution agr.toStatic; asimp at tyn
     rw[show B.[m.[σ] .: σ] = B.[up σ].[m.[σ]/] by asimp] at tyn
-    have ty := Typed.tup_im tyS tym tyn; assumption
-  case tup_ex B m n s i mrg tyS tym tyn ihm ihn =>
+    have er := Erased.tup_im tyS erm tyn; assumption
+  case tup_ex B m m' n n' s i mrg tyS erm ern ihm ihn =>
     have ⟨Δa, Δb, mrg, agr1, agr2⟩ := agr.split mrg
     replace tyS := tyS.substitution agr.toStatic; asimp at tyS
-    replace tym := ihm agr1; asimp at tym
-    replace tyn := ihn agr2; asimp at tyn
-    rw[show B.[m.[σ] .: σ] = B.[up σ].[m.[σ]/] by asimp] at tyn
-    have ty := Typed.tup_ex mrg tyS tym tyn; assumption
-  case proj_im A B C m n rA s sA sB sC iC rs mrg tyC tym tyn ihm ihn =>
+    replace erm := ihm agr1; asimp at erm
+    replace ern := ihn agr2; asimp at ern
+    rw[show B.[m.[σ] .: σ] = B.[up σ].[m.[σ]/] by asimp] at ern
+    have er := Erased.tup_ex mrg tyS erm ern; assumption
+  case proj_im A B C m m' n n' rA s sA sB sC iC c rs mrg tyC erm ern ihm ihn =>
     have ⟨_, _, _, tyS⟩ := tyC.ctx_inv
-    obtain ⟨_, _ | ⟨tyA, _⟩, tyB⟩ := tyn.ctx_inv
+    obtain ⟨_, _ | ⟨tyA, _⟩, tyB⟩ := ern.ctx_inv
     have ⟨Δa, Δb, mrg, agr1, agr2⟩ := agr.split mrg
     replace tyC := tyC.substitution (agr.toStatic.cons tyS); asimp at tyC
-    replace tym := ihm agr1; asimp at tym
-    replace tyn := ihn ((agr2.cons rA tyA).cons .im tyB); asimp at tyn
+    replace erm := ihm agr1; asimp at erm
+    replace ern := ihn ((agr2.cons rA tyA).cons .im tyB); asimp at ern
     rw[show C.[m.[σ] .: σ] = C.[up σ].[m.[σ]/] by asimp]
-    apply Typed.proj_im <;> (asimp; assumption)
-  case proj_ex C m n rA rB s sA sB sC i rs1 rs2 mrg tyC tym tyn ihm ihn =>
+    apply Erased.proj_im <;> (asimp; assumption)
+  case proj_ex C m m' n n' rA rB s sA sB sC i c1 c2 rs1 rs2 mrg tyC erm ern ihm ihn =>
     have ⟨_, _, _, tyS⟩ := tyC.ctx_inv
-    obtain ⟨_, _ | ⟨tyA, _⟩, tyB⟩ := tyn.ctx_inv
+    obtain ⟨_, _ | ⟨tyA, _⟩, tyB⟩ := ern.ctx_inv
     have ⟨Δa, Δb, mrg, agr1, agr2⟩ := agr.split mrg
     replace tyC := tyC.substitution (agr.toStatic.cons tyS); asimp at tyC
-    replace tym := ihm agr1; asimp at tym
-    replace tyn := ihn ((agr2.cons rA tyA).cons rB tyB); asimp at tyn
+    replace erm := ihm agr1; asimp at erm
+    replace ern := ihn ((agr2.cons rA tyA).cons rB tyB); asimp at ern
     rw[show C.[m.[σ] .: σ] = C.[up σ].[m.[σ]/] by asimp]
-    apply Typed.proj_ex
+    apply Erased.proj_ex
     . apply rs1
     . apply rs2
     . assumption
     . assumption
     . assumption
     . asimp; assumption
-  case tt h ih => constructor <;> aesop (rule_sets := [subst])
-  case ff h ih => constructor <;> aesop (rule_sets := [subst])
-  case ite A m n1 n2 s i mrg tyA tym tyn1 tyn2 ihm ihn1 ihn2 =>
+  case tt h ih => constructor; apply agr.wf h; apply agr.implicit ih
+  case ff h ih => constructor; apply agr.wf h; apply agr.implicit ih
+  case ite A m m' n1 n1' n2 n2' s i mrg tyA erm ern1 ern2 ihm ihn1 ihn2 =>
     have ⟨s, i, _, tyb⟩ := tyA.ctx_inv
     have ⟨Δ1', Δ2', mrg, agr1, agr2⟩ := agr.split mrg
     specialize ihm agr1; asimp at ihm
@@ -328,46 +286,44 @@ lemma Typed.substitution {Γ Γ'} {Δ Δ' : Ctx Srt} {A m σ} :
     replace tyA := tyA.substitution (agr.toStatic.cons tyb); asimp at tyA
     rw[show A.[.tt .: σ] = A.[up σ].[.tt/] by asimp] at ihn1
     rw[show A.[.ff .: σ] = A.[up σ].[.ff/] by asimp] at ihn2
-    have ty := Typed.ite mrg tyA ihm ihn1 ihn2; asimp at ty
+    have er := Erased.ite mrg tyA ihm ihn1 ihn2; asimp at er
     assumption
-  case rw A B m n a b s i tyA tym tyn ih =>
+  case rw A B m m' n a b s i tyA erm tyn ih =>
     have ⟨_, _, _, tyI⟩ := tyA.ctx_inv
     have ⟨_, _, _, tyB⟩ := tyI.ctx_inv
     replace tyA := tyA.substitution ((agr.toStatic.cons tyB).cons tyI); asimp at tyA
-    replace tym := ih agr; asimp at tym
+    replace erm := ih agr; asimp at erm
     replace tyn := tyn.substitution agr.toStatic; asimp at tyn
     simp[<-SubstLemmas.subst_comp] at tyA
     rw[show A.[a.[σ].rfl .: a.[σ] .: σ]
           = A.[upn 2 σ].[.rfl a.[σ],a.[σ]/]
-         by asimp] at tym
-    have := Typed.rw tyA tym tyn
+         by asimp] at erm
+    have := Erased.rw tyA erm tyn
     asimp at this; assumption
-  case conv eq tym tyB ih =>
+  case conv eq erm tyB ih =>
     replace tyB := tyB.substitution agr.toStatic
-    replace tym := ih agr
-    apply Typed.conv
-    . apply Conv.subst _ eq
+    replace erm := ih agr
+    apply Erased.conv
+    . apply Static.Conv.subst _ eq
     . assumption
     . assumption
-  case nil agr => apply agr.wf_nil
-  case cons agr => apply agr.wf_cons <;> aesop
 
-lemma Typed.subst_im {Γ} {Δ : Ctx Srt} {A B m n s} :
-    A :: Γ ;; A :⟨.im, s⟩ Δ ⊢ m : B ->
+lemma Erased.subst_im {Γ} {Δ : Ctx Srt} {A B m m' n s} :
+    A :: Γ ;; A :⟨.im, s⟩ Δ ⊢ m ▷ m' : B ->
     Γ ⊢ n : A ->
-    Γ ;; Δ ⊢ m.[n/] : B.[n/] := by
-  intro tym tyn
-  obtain ⟨_, _, _⟩ := tym.ctx_inv
-  apply tym.substitution
+    Γ ;; Δ ⊢ m.[n/] ▷ m'.[.none/] : B.[n/] := by
+  intro erm tyn
+  obtain ⟨_, _, _⟩ := erm.ctx_inv
+  apply erm.substitution
   apply AgreeSubst.wk_im
   . asimp; assumption
   . apply AgreeSubst.refl; assumption
 
-lemma Typed.subst_ex {Γ} {Δ1 Δ2 Δ : Ctx Srt} {A B m n s} :
+lemma Erased.subst_ex {Γ} {Δ1 Δ2 Δ : Ctx Srt} {A B m m' n n' s} :
     Δ2 ≤* s -> Merge Δ1 Δ2 Δ ->
-    A :: Γ ;; A :⟨.ex, s⟩ Δ1 ⊢ m : B ->
-    Γ ;; Δ2 ⊢ n : A ->
-    Γ ;; Δ ⊢ m.[n/] : B.[n/] := by
+    A :: Γ ;; A :⟨.ex, s⟩ Δ1 ⊢ m ▷ m' : B ->
+    Γ ;; Δ2 ⊢ n ▷ n' : A ->
+    Γ ;; Δ ⊢ m.[n/] ▷ m'.[n'/] : B.[n/] := by
   intro lw mrg tym tyn
   obtain ⟨_, _, _⟩ := tym.ctx_inv
   apply tym.substitution
@@ -377,33 +333,35 @@ lemma Typed.subst_ex {Γ} {Δ1 Δ2 Δ : Ctx Srt} {A B m n s} :
   . asimp; assumption
   . apply AgreeSubst.refl; assumption
 
-lemma Typed.esubst_im {Γ} {Δ : Ctx Srt} {A B B' m m' n s} :
-    m' = m.[n/] ->
-    B' = B.[n/] ->
-    A :: Γ ;; A :⟨.im, s⟩ Δ ⊢ m : B ->
+lemma Erased.esubst_im {Γ} {Δ : Ctx Srt} {A B1 B2 m1 m2 e1 e2 n s} :
+    m2 = m1.[n/] ->
+    e2 = e1.[.none/] ->
+    B2 = B1.[n/] ->
+    A :: Γ ;; A :⟨.im, s⟩ Δ ⊢ m1 ▷ e1 : B1 ->
     Γ ⊢ n : A ->
-    Γ ;; Δ ⊢ m' : B' := by
-  intros; subst_vars; apply Typed.subst_im <;> assumption
+    Γ ;; Δ ⊢ m2 ▷ e2 : B2 := by
+  intros; subst_vars; apply Erased.subst_im <;> assumption
 
-lemma Typed.esubst_ex {Γ} {Δ1 Δ2 Δ : Ctx Srt} {A B B' m m' n s} :
-    m' = m.[n/] ->
-    B' = B.[n/] ->
+lemma Erased.esubst_ex {Γ} {Δ1 Δ2 Δ : Ctx Srt} {A B1 B2 m1 e1 m2 e2 n1 n2 s} :
+    m2 = m1.[n1/] ->
+    e2 = e1.[n2/] ->
+    B2 = B1.[n1/] ->
     Δ2 ≤* s -> Merge Δ1 Δ2 Δ ->
-    A :: Γ ;; A :⟨.ex, s⟩ Δ1 ⊢ m : B ->
-    Γ ;; Δ2 ⊢ n : A ->
-    Γ ;; Δ ⊢ m' : B' := by
-  intros; subst_vars; apply Typed.subst_ex <;> assumption
+    A :: Γ ;; A :⟨.ex, s⟩ Δ1 ⊢ m1 ▷ e1 : B1 ->
+    Γ ;; Δ2 ⊢ n1 ▷ n2 : A ->
+    Γ ;; Δ ⊢ m2 ▷ e2 : B2 := by
+  intros; subst_vars; apply Erased.subst_ex <;> assumption
 
-lemma Typed.conv_ctx {Γ} {Δ : Ctx Srt} {A B C m r s i} :
+lemma Erased.conv_ctx {Γ} {Δ : Ctx Srt} {A B C m m' r s i} :
     B === A ->
     Γ ⊢ B : .srt s i ->
-    A :: Γ ;; A :⟨r, s⟩ Δ ⊢ m : C ->
-    B :: Γ ;; B :⟨r, s⟩ Δ ⊢ m : C := by
-  intro eq tyB tym
-  obtain ⟨_, wf, tyA⟩ := tym.ctx_inv
-  replace tym : B :: Γ ;; B :⟨r, s⟩ Δ ⊢ m.[ids] : C.[ids] := by
-    apply tym.substitution
+    A :: Γ ;; A :⟨r, s⟩ Δ ⊢ m ▷ m' : C ->
+    B :: Γ ;; B :⟨r, s⟩ Δ ⊢ m ▷ m' : C := by
+  intro eq tyB erm
+  obtain ⟨_, wf, tyA⟩ := erm.ctx_inv
+  replace erm : B :: Γ ;; B :⟨r, s⟩ Δ ⊢ m.[ids] ▷ m'.[ids] : C.[ids] := by
+    apply erm.substitution
     apply AgreeSubst.conv <;> try assumption
     . asimp; apply tyA.weaken tyB
     . apply AgreeSubst.refl; constructor <;> assumption
-  asimp at tym; assumption
+  asimp at erm; assumption
